src/CoreRules/CoreRules.v
@@ -7,3 +7,4 @@ Require Export CoreAutomation.
 Require Export XRules.
 Require Export ZXRules.
 Require Export SwapRules.
+Require Export PermutationRules.
